cava/cava/Cava/Arrow/Instances/Netlist.v
@@ -36,7 +36,7 @@ Section NetlistEval.
 
   #[refine] Instance NetlistCat : Category := {
     object := bundle;
-    morphism X Y := signalTy Signal X -> state (Netlist * N) (signalTy Signal Y);
+    morphism X Y := signalTy Signal X -> state CavaState (signalTy Signal Y);
     id X x := ret x;
     compose X Y Z f g := g >=> f;
 
@@ -124,68 +124,67 @@ Section NetlistEval.
       | false => Gnd
     end) n n v);
 
-    not_gate '(x,tt) :=
-      '(nl, i) <- get ;;
-      put (cons (Not x (Wire i)) nl, (i+1)%N) ;;
-      ret (Wire i);
+    not_gate '(i,tt) :=
+      o <- newWire ;;
+      addInstance (Not i o) ;;
+      ret o;
 
-    and_gate '(x,(y,tt)) :=
-      '(nl, i) <- get ;;
-      put (cons (And x y (Wire i)) nl, (i+1)%N) ;;
-      ret (Wire i);
+    and_gate '(i0,(i1,tt)) :=
+      o <- newWire ;;
+      addInstance (And i0 i1 o) ;;
+      ret o;
 
-    nand_gate '(x,(y,tt)) :=
-      '(nl, i) <- get ;;
-      put (cons (Nand x y (Wire i)) nl, (i+1)%N) ;;
-      ret (Wire  i);
+    nand_gate '(i0,(i1,tt)) :=
+      o <- newWire ;;
+      addInstance (Nand i0 i1 o) ;;
+      ret o;
 
-    or_gate '(x,(y,tt)) :=
-      '(nl, i) <- get ;;
-      put (cons (Or x y (Wire i)) nl, (i+1)%N) ;;
-      ret (Wire i);
+    or_gate '(i0,(i1,tt)) :=
+      o <- newWire ;;
+      addInstance (Or i0 i1 o) ;;
+      ret o;
 
-    nor_gate '(x,(y,tt)) :=
-      '(nl, i) <- get ;;
-      put (cons (Nor x y (Wire i)) nl, (i+1)%N) ;;
-      ret (Wire i);
+    nor_gate '(i0,(i1,tt)) :=
+      o <- newWire ;;
+      addInstance (Nor i0 i1 o) ;;
+      ret o;
 
-    xor_gate '(x,(y,tt)) :=
-      '(nl, i) <- get ;;
-      put (cons (Xor x y (Wire i)) nl, (i+1)%N) ;;
-      ret (Wire i);
+    xor_gate '(i0,(i1,tt)) :=
+      o <- newWire ;;
+      addInstance (Xor i0 i1 o) ;;
+      ret o;
 
-    xnor_gate '(x,(y,tt)) :=
-      '(nl, i) <- get ;;
-      put (cons (Xnor x y (Wire i)) nl, (i+1)%N) ;;
-      ret (Wire i);
+    xnor_gate '(i0,(i1,tt)) :=
+      o <- newWire ;;
+      addInstance (Xnor i0 i1 o) ;;
+      ret o;
 
-    buf_gate '(x,tt) :=
-      '(nl, i) <- get ;;
-      put (cons (Buf x (Wire i)) nl, (i+1)%N) ;;
-      ret (Wire i);
+    buf_gate '(i,tt) :=
+      o <- newWire ;;
+      addInstance (Buf i o) ;;
+      ret o;
 
-    xorcy '(x, (y, tt)) :=
-      '(nl, i) <- get ;;
-      put (cons (Component "XORCY" [] [("O", Wire i); ("CI", x); ("LI", y)]) nl, (i+1)%N) ;;
-      ret (Wire i);
+    xorcy '(i0, (i1, tt)) :=
+      o <- newWire ;;
+      addInstance (Component "XORCY" [] [("O", o); ("CI", i0); ("LI", i1)]) ;;
+      ret o;
 
     muxcy '(s,(ci,(di, tt))) :=
-      '(nl, i) <- get ;;
-      put (cons (Component "MUXCY" [] [("O", Wire i); ("S", s); ("CI", ci); ("DI", di)]) nl, (i+1)%N) ;;
-      ret (Wire i);
+      o <- newWire ;;
+      addInstance ( Component "MUXCY" [] [("O", o); ("S", s); ("CI", ci); ("DI", di)]) ;;
+      ret o;
 
     unsigned_add m n s '(x,(y, tt)) :=
-      '(nl, i) <- get ;;
-      let o := map N.of_nat (seq (N.to_nat i) s) in
-      put (cons (UnsignedAdd x y (map Wire o)) nl, (i + N.of_nat s)%N) ;;
-      ret (map Wire o);
+      sum <- newWires s ;;
+      addInstance (UnsignedAdd x y sum) ;;
+      ret sum;
   }.
 
   Close Scope string_scope.
 
   Fixpoint map2WithPortShape {A B C} (f: A -> B -> C) (port: Kind)
     (x: denoteKindWith port A) (y: denoteKindWith port B): denoteKindWith port C :=
-    match port in Kind, x, y return  denoteKindWith port C with
+    match port in Kind, x, y return denoteKindWith port C with
     | Bit, x, y => f x y
     | BitVec sz, xs, ys => mapBitVec (fun '(x,y) => f x y) sz sz (zipBitVecs sz sz xs ys)
     end .
@@ -202,44 +201,19 @@ Section NetlistEval.
         (linkShapes link s2 p12 p22)
     end.
 
-  Definition bitsInPortShape' i s := (i + N.of_nat (bitsInPortShape s))%N.
-
   Instance NetlistLoop : ArrowLoop NetlistArr := {
-    (* 1. reserve (@numberShape N _) items
-       2. Run f with reserved items
-       3. link the items and add the netlist *)
-    loopr _ _ N f x :=
-      (* 1 *)
-      '(nl, i) <- get ;;
-      let n := numberPort i N in
-      let i' := bitsInPortShape' i N in
-      put (nl, i') ;;
-
-      (* 2 *)
-      '(y,n') <- f (x,n) ;;
-
-      (* 3 *)
-      let links := linkShapes AssignBit N n n' in
-      '(nl, i) <- get ;;
-      put (links ++ nl, i) ;;
-
+    loopr _ _ Z f x :=
+      z <- newWiresFromShape Z ;;
+      '(y,z') <- f (x,z) ;;
+      let links := linkShapes AssignBit Z z z' in
+      addSequentialInstances links;;
       ret y;
 
-    loopl _ _ N f x :=
-      (* 1 *)
-      '(nl, i) <- get ;;
-      let n := numberPort i N in
-      let i' := bitsInPortShape' i N in
-      put (nl, i') ;;
-
-      (* 2 *)
-      '(n', y) <- f (n, x) ;;
-
-      (* 3 *)
-      let links := linkShapes AssignBit N n n' in
-      '(nl, i) <- get ;;
-      put (links ++ nl, i) ;;
-
+    loopl _ _ Z f x :=
+      z <- newWiresFromShape Z ;;
+      '(z',y) <- f (z,x) ;;
+      let links := linkShapes AssignBit Z z z' in
+      addSequentialInstances links;;
       ret y;
   }.
 
@@ -247,95 +221,10 @@ Section NetlistEval.
     delay_cava := NetlistCava;
 
     delay_gate X '(x,tt) :=
-      '(nl, i) <- get ;;
-      let x' := numberPort i X in
-      let i' := bitsInPortShape' i X in
-      let links := linkShapes DelayBit X x x' in
-      put (links ++ nl, i') ;;
-      ret x'
+      y <- newWiresFromShape X ;;
+      let links := linkShapes DelayBit X x y in
+      addSequentialInstances links;;
+      ret y;
   }.
-
-  Definition wireInput (port_shape: Kind) (name: string) (port: denoteKindWith port_shape Signal)
-    : Instance :=
-    match port_shape, port with
-    | Bit,_ => WireInputBit name port
-    | BitVec sz,_ => WireInputBitVec sz name port
-    end.
-
-  Definition wireOutput (port_shape: Kind) (name: string) (port: denoteKindWith port_shape Signal)
-    : Instance :=
-    match port_shape, port with
-    | Bit,_ => WireOutputBit name port
-    | BitVec sz,_ => WireOutputBitVec sz name port
-    end.
-
-  Fixpoint nameTy {A} (s : @shape A) : Type :=
-    match s with
-    | Empty  => Datatypes.unit
-    | One t => string
-    | Tuple2 s1 s2  => prod (nameTy s1) (nameTy s2)
-    end.
-
-  Fixpoint linkLables {A}
-     (link: forall port_shape, string -> denoteKindWith port_shape Signal -> A)
-     (s: shape)
-     (labels: nameTy s)
-     (ports: signalTy Signal s)
-     : list A :=
-    match s in shape, labels, ports with
-    | Empty, _, _ => []
-    | One port_shape, name, port => [link port_shape name port]
-    | Tuple2 s1 s2, (l1,l2), (p1,p2) => (linkLables link s1 l1 p1) ++ (linkLables link s2 l2 p2)
-    end.
-
-  Fixpoint namePorts
-     (s: bundle)
-     (labels: nameTy s)
-     : list PortDeclaration :=
-    match s in shape, labels with
-    | Empty, _ => []
-    | One port_shape, name => [mkPort name port_shape]
-    | Tuple2 s1 s2, (l1,l2) => (namePorts s1 l1) ++ (namePorts s2 l2)
-    end.
-
-  Definition nameInputs {X}
-    (input_names: nameTy X)
-    : X ~[NetlistCat]~> X :=
-      fun x =>
-        '(nl, i) <- get ;;
-        let links := linkLables wireInput X input_names x in
-        put (links ++ nl, i) ;;
-        ret x.
-
-  Definition nameOutputs {X}
-    (output_names: nameTy X)
-    : X ~[NetlistCat]~> X :=
-      fun x =>
-        '(nl, i) <- get ;;
-        let links := linkLables wireOutput X output_names x in
-        put (links ++ nl, i) ;;
-        ret x.
-
-  Definition arrowToHDLModule {X Y}
-    (name: string)
-    (f: X ~[NetlistCat]~> Y)
-    (input_names: nameTy X)
-    (output_names: nameTy Y)
-    : Netlist.CavaState :=
-      let i := numberPort 2 X in
-      let n := bitsInPortShape' 2 X in
-      let '(o, (netlist, count)) := runState ((nameInputs input_names >=> f >=> nameOutputs output_names) i) ([], n) in
-      let module_inputs := namePorts X input_names in
-      let module_ouputs := namePorts Y output_names in
-      let module := mkModule name netlist module_inputs module_ouputs in
-      mkCavaState count true module.
-
-  (* Check ArrowExamples.v for xor example *)
-  Local Open Scope string_scope.
-  Eval cbv in arrowToHDLModule
-    "not"
-    not_gate
-    ("input1", tt)
-    ("output1").
 
 End NetlistEval.
